\documentclass[notes=only]{beamer}
\setbeamertemplate{note page}[plain]

\begin{document}

\note[itemize]
%Diagonalisierbar
{
	\item Diagonalisierbar $->$
	\item $w_1^+ = \lambda_1 w_1; w_2^+ = \lambda_2 w_2$
	\item $\lambda$ kompensieren:
	\item $\varrho_{1,2} = \frac{1}{2\pi i}log(\lambda_{1,2})$
	\item $z^{\varrho_{1,2}} = e^{log(z^{\varrho_{1,2}})} = e^{\varrho_{1,2} log(z)}$
	\item Analytisch Fortsetzen...
	\item $e^{\varrho_{1,2} log(z)}  \text{@}  e^{\varrho_{1,2} (log(z) + 2\pi i)}
			= e^{\varrho_{1,2} log(z)}  e^{2\pi i\frac{1}{2\pi i}log(\lambda_{1,2})}
			= z^{\varrho_{1,2}}  \lambda_{1,2}$
	\item Verhaeltnis bilden...
	\item $\frac{w_{1,2}}{z^\varrho_{1,2}} @
		\frac{\lambda_{1,2}w_{1,2}}{\lambda_{1,2}z^{\varrho_{1,2}}}
		=\frac{w_{1,2}}{z^{\varrho_{1,2}}} = \mathcal{L}(z)$
	\item $w_{1,2} = z^{\varrho_{1,2}}\mathcal{L}(z)$
	\item Schon bekannt, beweis
	
}
\note[itemize]
%Jordan-Normalform
{
	\item nicht diagonalisierbar $->$
	\item $w_2 = \lambda_2*w_2 + w_1$
	\item $\frac{w_2}{w_1} @ \frac{\lambda w_2}{\lambda w_1} = \frac{w_2}{2_1}
		+ \frac{1}{\lambda}$
	\item $\frac{1}{\lambda}$ kompensieren
	\item $\frac{1}{2\pi i\lambda} log(z) @\frac{1}{2\pi i\lambda} log(z)
		 +  \frac{1}{\lambda}$
	\item Verhaeltnis...
	\item $\frac{w_2}{w_1} - \frac{1}{2\pi i\lambda} log(z)
		@ \frac{w_2}{w_1} - \frac{1}{2\pi i\lambda} log(z) = \mathcal{L}(z)$
	\item Aufloesen...
	\item $w_2 = \mathcal{L}_1w_1 + aw_1log(z) = z^{\varrho_1}\mathcal{L}_2 + aw_1log(z)$
	\item $\mathcal{L}\mathcal{L}=\mathcal{L}$
}
\end{document}}